allow for different stages to have different numbers of levels; add a stage argument to [get_index] and thread that through everywhere else

coq-verification/src/Concrete/Assumptions/PageTables.v
@@ -15,7 +15,9 @@
  *)
 
 Require Import Coq.Lists.List.
+Require Import Coq.NArith.BinNat.
 Require Import Hafnium.Concrete.Datatypes.
+Require Import Hafnium.Concrete.Notations.
 Require Import Hafnium.Concrete.Assumptions.Addr.
 Require Import Hafnium.Concrete.Assumptions.ArchMM.
 Require Import Hafnium.Concrete.Assumptions.Constants.
@@ -26,15 +28,6 @@ Require Import Hafnium.Concrete.MM.Datatypes.
      be considered part of the TCB, because the proofs rely on this transcription
      being a correct description of the lookup procedure. ***)
 
-(* index in each level of the page table (highest is root) *)
-Axiom index0 : uintpaddr_t -> nat.
-Axiom index1 : uintpaddr_t -> nat.
-Axiom index2 : uintpaddr_t -> nat.
-Axiom index3 : uintpaddr_t -> nat.
-
-(* in-page offset *)
-Axiom offset : uintpaddr_t -> nat.
-
 (* if we have a table PTE, we want to extract the address and get a
    ptable_pointer out of it *)
 Axiom ptable_pointer_from_address : paddr_t -> ptable_pointer.
@@ -42,14 +35,59 @@ Axiom ptable_pointer_from_address : paddr_t -> ptable_pointer.
 Definition get_entry (ptable : mm_page_table) (i : nat) : option pte_t :=
   nth_error ptable.(entries) i.
 
-Definition get_index (level : nat) (a : uintpaddr_t) : nat :=
-  match level with
-  | 0 => index0 a
-  | 1 => index1 a
-  | 2 => index2 a
-  | 3 => index3 a
-  | _ => 0 (* invalid level *)
+Axiom get_stage1_index : nat (* level *) -> uintpaddr_t -> nat.
+Axiom get_stage2_index : nat (* level *) -> uintpaddr_t -> nat.
+
+(* enum for stages 1 and 2 *)
+Inductive Stage : Type := Stage1 | Stage2.
+
+Definition get_index (s : Stage) (level : nat) (a : uintpaddr_t) : nat :=
+  match s with
+  | Stage1 => get_stage1_index level a
+  | Stage2 => get_stage2_index level a
   end.
+
+Definition max_level (s : Stage) : nat :=
+  match s with
+  | Stage1 => arch_mm_stage1_max_level
+  | Stage2 => arch_mm_stage2_max_level
+  end.
+
+Definition is_stage1 (s : Stage) : bool :=
+  match s with
+  | Stage1 => true
+  | Stage2 => false
+  end.
+
+Axiom stage1_index_of_uintvaddr :
+  forall (a : uintvaddr_t) (level : nat),
+    (* level offset for uintvaddr_t *)
+    let offset := (PAGE_BITS + level * PAGE_LEVEL_BITS)%N in
+    (* convert a to uintpaddr_t *)
+    let b : uintpaddr_t := pa_addr (pa_from_va (va_init a)) in
+    level <= S (max_level Stage1) ->
+    get_stage1_index level b = N.to_nat ((a / 2 ^ offset) mod 2 ^ PAGE_LEVEL_BITS).
+
+Axiom stage2_index_of_uintvaddr :
+  forall (a : uintvaddr_t) (level : nat),
+    (* level offset for uintvaddr_t *)
+    let offset := (PAGE_BITS + level * PAGE_LEVEL_BITS)%N in
+    (* convert a to uintpaddr_t *)
+    let b : uintpaddr_t := pa_addr (pa_from_va (va_init a)) in
+    level <= S (max_level Stage2) ->
+    get_stage2_index level b = N.to_nat ((a / 2 ^ offset) mod 2 ^ PAGE_LEVEL_BITS).
+
+(* TODO: this limits level to [S (max_level stage)] to allow for indices in
+   top-level lists of root tables -- is that the correct behavior? *)
+Lemma index_of_uintvaddr (a : uintvaddr_t) (level : nat) stage :
+    let offset := (PAGE_BITS + level * PAGE_LEVEL_BITS)%N in
+    let b : uintpaddr_t := pa_addr (pa_from_va (va_init a)) in
+    level <= S (max_level stage) ->
+    get_index stage level b = N.to_nat ((a / 2 ^ offset) mod 2 ^ PAGE_LEVEL_BITS).
+Proof.
+  destruct stage; cbv [get_index];
+    auto using stage1_index_of_uintvaddr, stage2_index_of_uintvaddr.
+Qed.
 
 (* N.B. the [option] here doesn't mean whether the entry is
    valid/present; rather, the lookup should return [Some] for any
@@ -59,11 +97,12 @@ Fixpoint page_lookup'
          (a : uintpaddr_t)
          (table : mm_page_table)
          (level : nat)
+         (s : Stage)
   : option pte_t :=
   match level with
   | 0 => None
   | S level' =>
-    match (get_entry table (get_index level a)) with
+    match (get_entry table (get_index s level a)) with
     | Some pte =>
       if (arch_mm_pte_is_table pte level)
       then
@@ -71,7 +110,7 @@ Fixpoint page_lookup'
         let next_ptr := ptable_pointer_from_address
                           (arch_mm_table_from_pte pte level) in
         let next_table := ptable_deref next_ptr in
-        page_lookup' ptable_deref a next_table level'
+        page_lookup' ptable_deref a next_table level' s
       else Some pte
     | None => None
     end
@@ -79,6 +118,6 @@ Fixpoint page_lookup'
 
 Definition page_lookup
            (ptable_deref : ptable_pointer -> mm_page_table)
-           (root_ptable : ptable_pointer)
+           (root_ptable : ptable_pointer) (s : Stage)
            (a : uintpaddr_t) : option pte_t :=
-  page_lookup' ptable_deref a (ptable_deref root_ptable) 4.
+  page_lookup' ptable_deref a (ptable_deref root_ptable) (max_level s) s.
